coq_session/dyn_prog.v
@@ -1,0 +1,32 @@
+From mathcomp Require Import ssreflect ssrbool eqtype ssrnat seq.
+From Coq Require Import ssrfun Classical Utf8.
+Require Export AutosubstSsr ARS dyn_inv.
+
+Lemma dyn_monad_canonical Θ v A T :
+  Θ ; nil ; nil ⊢ v : T -> dyn_val v -> IO A ≃ T ->
+  (exists u, dyn_val u ∧ v = Return u) ∨ (dyn_thunk v).
+Proof.
+  move e1:(nil)=>Γ.
+  move e2:(nil)=>Δ ty.
+  elim: ty A e1 e2=>//{Θ Γ Δ v T};
+  try solve[intros; exfalso; solve_conv].
+  { move=>Θ Γ Δ x s A emp wf hs1 hs2 A0 e1 e2 vl eq. subst. inv hs2. }
+  { intros. subst. inv H2. eauto. }
+  { intros. subst. inv H5. eauto. }
+  { intros. subst. inv H6. eauto. }
+  { intros. subst. inv H6. eauto. }
+  { intros. subst. inv H8. eauto. }
+  { intros. subst. inv H1.
+    left. exists m. eauto. inv H3. }
+  { intros. subst. inv H6. eauto. }
+  { intros. subst. inv H1. eauto. }
+  { intros. subst. inv H2. eauto. }
+  { intros. subst. inv H2. eauto. }
+  { intros. subst. inv H1. eauto. }
+  { intros. subst. inv H1. eauto. }
+  { intros. subst.
+    apply: H1; eauto.
+    apply: conv_trans.
+    apply: H4.
+    apply: conv_sym; eauto. }
+Qed.
